Replacing tlt with binary primitive Lt + cleanup

Evaluator.v
@@ -30,104 +30,216 @@ Fixpoint is_value (t: tree) : bool :=
     | notype_lambda _ => true
     | _ => false end.
 
+Lemma is_value_correct : forall v, is_value v = true <-> cbv_value v.
+Proof.
+  split.
+  - induction v; repeat step || bools; eauto with values.
+  - induction 1; repeat step || bools.
+Defined.
+
+
 Definition get_pair t : {t': option (tree*tree) | forall t1 t2, t' = Some (t1, t2) <-> t = pp t1 t2}.
-  Proof.
-    exists ( match t with
-    | pp e1 e2 => Some (e1,e2)
-    | _ => None end).
-    destruct t; steps.
-  Defined.
+Proof.
+  exists ( match t with
+      | pp e1 e2 => Some (e1,e2)
+      | _ => None end).
+  destruct t; steps.
+Defined.
 
-  Definition get_app t : {t': option tree | forall t1, t' = Some t1 <-> t = notype_lambda t1}.
-  Proof.
-    exists (match t with
-       | notype_lambda body => Some body
-       | _ => None end).
-    destruct t; steps.
-  Defined.
+Definition get_app t : {t': option tree | forall t1, t' = Some t1 <-> t = notype_lambda t1}.
+Proof.
+  exists (match t with
+     | notype_lambda body => Some body
+     | _ => None end).
+  destruct t; steps.
+Defined.
 
-  Definition get_LR t : {t': option tree | forall t1, t' = Some t1 <-> (t = tleft t1 \/ t = tright t1)}.
-  Proof.
-    exists (match t with
-       | tleft t' => Some t'
-       | tright t' => Some t'
-       | _ => None end).
-    destruct t; steps.
-  Defined.
+Definition get_LR t : {t': option tree | forall t1, t' = Some t1 <-> (t = tleft t1 \/ t = tright t1)}.
+Proof.
+  exists (match t with
+     | tleft t' => Some t'
+     | tright t' => Some t'
+     | _ => None end).
+  destruct t; steps.
+Defined.
+
+Fixpoint get_nat t :=
+  match t with
+  | zero => Some 0
+  | succ t => option_map S (get_nat t)
+  | _ => None
+  end.
+
+Lemma get_nat_build_nat :
+  forall n, get_nat (build_nat n) = Some n.
+Proof.
+  induction n; repeat steps || rewrite_any.
+Qed.
+
+Lemma get_nat_prop :
+  forall t n, get_nat t = Some n -> t = build_nat n.
+Proof.
+  induction t; steps.
+  destruct n; unfold option_map in *; steps.
+Qed.
+
+
+Definition ss_eval_binary_primitive (o:op) t1 t2 :=
+  match (get_nat t1), (get_nat t2) with
+  | (Some n1), (Some n2) => (
+      match o with
+      | Eq => Some (if (PeanoNat.Nat.eqb n1 n2) then ttrue else tfalse)
+      | Neq => Some (if (PeanoNat.Nat.eqb n1 n2) then tfalse else ttrue)
+      | Plus => Some (build_nat (n1 + n2))
+      | Minus => if (PeanoNat.Nat.leb n2 n1) then
+                  Some (build_nat (Nat.sub n1 n2))
+                else None
+      | Mul => Some (build_nat (n1 * n2))
+      | Div => if (PeanoNat.Nat.ltb 0 n2) then
+                Some (build_nat (PeanoNat.Nat.div n1 n2))
+              else None
+      | Lt => Some (if (PeanoNat.Nat.ltb n1 n2) then ttrue else tfalse)
+      | Leq => Some (if (PeanoNat.Nat.leb n1 n2) then ttrue else tfalse)
+      | Gt => Some (if (PeanoNat.Nat.leb n1 n2) then tfalse else ttrue)
+      | Geq => Some (if (PeanoNat.Nat.ltb n1 n2) then tfalse else ttrue)
+      | And | Or | Not | Cup | Nop => None  end)
+  | _, _ => match o,t1,t2 with
+           | And, ttrue, ttrue => Some ttrue
+           | And, ttrue, tfalse => Some tfalse
+           | And, tfalse, ttrue => Some tfalse
+           | And, tfalse, tfalse => Some tfalse
+           | Or, ttrue, ttrue => Some ttrue
+           | Or, ttrue, tfalse => Some ttrue
+           | Or, tfalse, ttrue => Some ttrue
+           | Or, tfalse, tfalse => Some tfalse
+           | _,_,_ => None end
+  end.
+
+Opaque PeanoNat.Nat.leb.
+Opaque PeanoNat.Nat.ltb.
+
+Ltac natb_rewrites :=
+  repeat rewrite PeanoNat.Nat.leb_le in * || rewrite PeanoNat.Nat.ltb_lt in * || rewrite PeanoNat.Nat.eqb_eq in * || rewrite PeanoNat.Nat.eqb_neq in * || rewrite PeanoNat.Nat.ltb_nlt in * || rewrite PeanoNat.Nat.leb_nle in *.
+
+Lemma ss_eval_binary_primitive_prop :
+  forall o t1 t2 t,
+    cbv_value t1 ->
+    cbv_value t2 ->
+    ss_eval_binary_primitive o t1 t2 = Some t <-> scbv_step (binary_primitive o t1 t2) t.
+Proof.
+  split; intros.
+  + unfold ss_eval_binary_primitive in *; steps;
+      repeat apply_anywhere get_nat_prop ; subst ;
+        eapply scbv_step_same; try constructor ; repeat steps || natb_rewrites.
+  + t_invert_step; steps.
+    all: try solve [
+               unfold ss_eval_binary_primitive;
+               repeat rewrite get_nat_build_nat in * || natb_rewrites || steps] .
+    all: try solve [
+               exfalso;
+               eauto using evaluate_step ].
+Qed.
+
+Lemma ss_eval_binary_primitive_prop2 :
+  forall o t1 t2 t,
+    is_value t1 = true ->
+    is_value t2 = true ->
+    ss_eval_binary_primitive o t1 t2 = Some t <-> scbv_step (binary_primitive o t1 t2) t.
+Proof.
+  intros. repeat rewrite is_value_correct in *. eauto using ss_eval_binary_primitive_prop.
+Qed.
 
 
 (* Evaluator (smallstep) *)
 Fixpoint ss_eval (t: tree) {struct t}: (option tree) :=
   match t with
-    | ite ttrue t1 t2 => Some t1
-    | ite tfalse t1 t2 => Some t2
-    | ite t t1 t2 => option_map (fun e => ite e t1 t2) (ss_eval t)
+  | ite ttrue t1 t2 => Some t1
+  | ite tfalse t1 t2 => Some t2
+  | ite t t1 t2 => option_map (fun e => ite e t1 t2) (ss_eval t)
 
-    | pp e1 e2 => match (is_value e1) with
-                   | true => option_map (pp e1) (ss_eval e2)
-                   | false => option_map (fun e => pp e e2) (ss_eval e1) end
+  | pp e1 e2 => match (is_value e1) with
+               | true => option_map (pp e1) (ss_eval e2)
+               | false => option_map (fun e => pp e e2) (ss_eval e1) end
 
-    | pi1 t => match get_pair t with
-              | exist _ None _  => option_map pi1 (ss_eval t)
-              | exist _ (Some (e1, e2)) _ =>
-                if (is_value e1) && (is_value e2)
-                then Some e1
-                else option_map pi1 (ss_eval t) end
+  | pi1 t => match get_pair t with
+            | exist _ None _  => option_map pi1 (ss_eval t)
+            | exist _ (Some (e1, e2)) _ =>
+              if (is_value e1) && (is_value e2)
+              then Some e1
+              else option_map pi1 (ss_eval t) end
 
-    | pi2 t => match get_pair t with
-              | exist _ None _ => option_map pi2 (ss_eval t)
-              | exist _ (Some (e1, e2)) _ =>
-                if (is_value e1) && (is_value e2)
-                then Some e2
-                else option_map pi2 (ss_eval t) end
+  | pi2 t => match get_pair t with
+            | exist _ None _ => option_map pi2 (ss_eval t)
+            | exist _ (Some (e1, e2)) _ =>
+              if (is_value e1) && (is_value e2)
+              then Some e2
+              else option_map pi2 (ss_eval t) end
 
-    | app t1 t2 => match (is_value t1) with
-                    | true => match get_app t1 with
-                             | exist _ None _ => option_map (app t1) (ss_eval t2)
-                             | exist _ (Some ts) _ =>
-                               if (is_value t2)
-                               then Some (open 0 ts t2)
-                               else option_map (app t1) (ss_eval t2) end
-                    | false => option_map (fun e => app e t2) (ss_eval t1) end
+  | app t1 t2 => match (is_value t1) with
+                | true => match get_app t1 with
+                         | exist _ None _ => option_map (app t1) (ss_eval t2)
+                         | exist _ (Some ts) _ =>
+                           if (is_value t2)
+                           then Some (open 0 ts t2)
+                           else option_map (app t1) (ss_eval t2) end
+                | false => option_map (fun e => app e t2) (ss_eval t1) end
 
-    | notype_tfix ts => Some (open 0 (open 1 ts zero) (notype_tfix ts))
+  | notype_tfix ts => Some (open 0 (open 1 ts zero) (notype_tfix ts))
 
-    | succ t => option_map succ (ss_eval t)
+  | succ t => option_map succ (ss_eval t)
 
-    | tmatch t1 t0 ts => match t1 with
-                       | zero => Some t0
-                       | succ t2 =>
-                         if (is_value t2)
-                         then Some (open 0 ts t2)
-                         else option_map (fun e => tmatch e t0 ts) (ss_eval t1)
-                       | _ => option_map (fun e => tmatch e t0 ts) (ss_eval t1) end
+  | tmatch t1 t0 ts => match t1 with
+                      | zero => Some t0
+                      | succ t2 =>
+                        if (is_value t2)
+                        then Some (open 0 ts t2)
+                        else option_map (fun e => tmatch e t0 ts) (ss_eval t1)
+                      | _ => option_map (fun e => tmatch e t0 ts) (ss_eval t1) end
 
-    | sum_match t tl tr => if (is_value t) then match t with
-                                   | tleft v => Some (open 0 tl v)
-                                   | tright v => Some (open 0 tr v)
+  | sum_match t tl tr => if (is_value t) then match t with
+                                             | tleft v => Some (open 0 tl v)
+                                             | tright v => Some (open 0 tr v)
+                                             | _ => None end
+                        else option_map (fun e => sum_match e tl tr) (ss_eval t)
+
+  | tleft t => option_map tleft (ss_eval t)
+  | tright t => option_map tright (ss_eval t)
+
+  | tsize t => if (is_value t) then Some (build_nat (tsize_semantics t)) else (option_map tsize (ss_eval t))
+  | boolean_recognizer r t => if (is_value t) then match r with
+                                                  | 0 => Some (is_pair t)
+                                                  | 1 => Some (is_succ t)
+                                                  | 2 => Some (is_lambda t)
+                                                  | _ => None end
+                             else option_map (boolean_recognizer r) (ss_eval t)
+
+  | unary_primitive o t => match (is_value t) with
+                          | false => option_map (unary_primitive o) (ss_eval t)
+                          | true => match o with
+                                   | Not => match t with
+                                           | ttrue => Some (tfalse)
+                                           | tfalse => Some (ttrue)
+                                           | _ => None end
                                    | _ => None end
-                          else option_map (fun e => sum_match e tl tr) (ss_eval t)
+                          end
 
-    | tleft t => option_map tleft (ss_eval t)
-    | tright t => option_map tright (ss_eval t)
+  | binary_primitive o t1 t2 => match (is_value t1) with
+                               | false => option_map (fun e => binary_primitive o e t2) (ss_eval t1)
+                               | true => match (is_value t2) with
+                                        | false => option_map (binary_primitive o t1) (ss_eval t2)
+                                        | true => ss_eval_binary_primitive o t1 t2 end
+                               end
 
-    | tsize t => if (is_value t) then Some (build_nat (tsize_semantics t)) else (option_map tsize (ss_eval t))
-    | boolean_recognizer r t => if (is_value t) then match r with
-                                                   | 0 => Some (is_pair t)
-                                                   | 1 => Some (is_succ t)
-                                                   | 2 => Some (is_lambda t)
-                                                   | _ => None end
-                               else option_map (boolean_recognizer r) (ss_eval t)
-    | _ => None
+  | _ => None
   end.
 
 (* Compute a certain number of small steps *)
 Fixpoint ss_eval_n (t : tree) (k: nat) : (option tree) :=
   match k with
-    | 0 => Some t
-    | S k' => match ss_eval t with
-               | Some t' => ss_eval_n t' k'
-               | None => Some t end
+  | 0 => Some t
+  | S k' => match ss_eval t with
+           | Some t' => ss_eval_n t' k'
+           | None => Some t end
   end.
 
 (* Entry point for evaluation *)
@@ -137,7 +249,7 @@ Definition eval (t: tree) (k: nat): (option tree) :=
 
 (* Tactics *)
 Ltac destruct_sig :=
-match goal with
+  match goal with
   | H: _ |- context[let _ := get_pair ?t in _ ]  =>
     let fresh := fresh "get_pair" in destruct (get_pair t) (* eqn:fresh *)
   | H: context[get_pair ?t = _ ] |- _ =>
@@ -148,21 +260,14 @@ match goal with
     let fresh := fresh "get_app" in destruct (get_app t) (* eqn:fresh *)
   | H: context[_ = get_app ?t ] |- _ =>
     let fresh := fresh "get_app" in destruct (get_app t) (* eqn:fresh *)
-end. (* match on type of t = sig *)
+  end. (* match on type of t = sig *)
 
 Ltac destruct_ss_eval :=
   match goal with
-    | H: context[ss_eval ?t] |- _ => destruct (ss_eval t) end.
+  | H: context[ss_eval ?t] |- _ => destruct (ss_eval t) end.
 
 
 (* Results *)
-Lemma is_value_correct : forall v, is_value v = true <-> cbv_value v.
-Proof.
-  split.
-  - induction v; repeat step || bools; eauto with values.
-  - induction 1; repeat step || bools.
-Defined.
-
 Lemma ss_eval_step : forall t t', ss_eval t = Some t' -> is_value t = true -> False.
 Proof.
   induction t; repeat step || options.
@@ -173,26 +278,59 @@ Ltac ss_eval_step :=
   |H: ss_eval ?t1 = Some ?t2 |- _ => poseNew (Mark (t1, t2) "ss_eval_step_h");
                                    pose proof  (ss_eval_step _ _ H) end.
 
+Lemma is_value_build_nat_false:
+  forall n,
+    is_value (build_nat n) = false -> False.
+Proof.
+  intros.
+  assert (is_value (build_nat n) = true ). rewrite is_value_correct; eauto with values.
+  steps.
+Qed.
+
+Ltac is_value_build_nat_false :=
+  match goal with
+  |H: is_value (build_nat ?n) = false |- _ => exfalso; apply (is_value_build_nat_false n H)
+  end.
 
 Lemma ss_eval_correct2: forall t t',
-  pfv t term_var = nil ->
-  t ~> t' ->
-  ss_eval t = Some t'.
+    pfv t term_var = nil ->
+    t ~> t' ->
+    ss_eval t = Some t'.
 Proof.
-  intros. induction H0 ; repeat light || options || invert_constructor_equalities || ss_eval_step || destruct_sig || instantiate_eq_refl || list_utils || bools || rewrite <- is_value_correct in * ||  eauto using fv_nil_top_level_var with smallstep values || destruct_match.
+  intros.
+  induction H0 ;
+    repeat light || options || invert_constructor_equalities
+    || ss_eval_step || destruct_sig || instantiate_eq_refl
+    || list_utils || bools
+    || (rewrite <- is_value_correct in * )
+    || (rewrite get_nat_build_nat in * )
+    || natb_rewrites
+    || is_value_build_nat_false
+    || (eauto using ss_eval_binary_primitive_prop2, fv_nil_top_level_var with smallstep values)
+    || destruct_match || unfold ss_eval_binary_primitive.
 Qed.
 
 Lemma ss_eval_correct1: forall t t',
-  ss_eval t = Some t' ->
-  pfv t term_var = nil ->
-  t ~> t'.
+    ss_eval t = Some t' ->
+    pfv t term_var = nil ->
+    t ~> t'.
 Proof.
-  induction t; intros ; repeat light ; destruct_ss_eval ; repeat light || options || bools || list_utils || instantiate_eq_refl || invert_constructor_equalities || rewrite is_value_correct in * || destruct_sig || congruence ||  step_inversion cbv_value || destruct_match ; eauto using ss_eval_step, fv_nil_top_level_var with smallstep values.
+  induction t;
+    intros ;
+    repeat light ; destruct_ss_eval ;
+      repeat light || options || bools
+      || list_utils || instantiate_eq_refl || invert_constructor_equalities
+      || (rewrite is_value_correct in *)
+         || destruct_sig || congruence
+         ||  step_inversion cbv_value || destruct_match ;
+         eauto using ss_eval_binary_primitive_prop2, ss_eval_step, fv_nil_top_level_var with smallstep values.
+         all: try solve [
+                    apply ss_eval_binary_primitive_prop; eauto ].
 Qed.
 
 (* Main theorem : the evaluator corresponds to the small call-by-value steps *)
 Theorem ss_eval_correct : forall t t',
-  pfv t term_var = nil ->
+    pfv t term_var = nil ->
     ss_eval t = Some t' <-> t ~> t'.
 Proof.
   split; eauto using ss_eval_correct1, ss_eval_correct2.
@@ -206,4 +344,4 @@ Extraction Language Ocaml.
 Set Extraction AccessOpaque.
 
 Extraction "evaluator.ml" eval.
-*)
+ *)
