AnnotatedFix.v
@@ -3,7 +3,6 @@ Require Import Coq.Lists.List.
 Require Export SystemFR.Judgments.
 Require Export SystemFR.AnnotatedTactics.
 Require Export SystemFR.ErasedFix.
-Require Export SystemFR.NatLessThanErase.
 
 Opaque reducible_values.
 
@@ -31,7 +30,7 @@ Lemma annotated_reducible_fix_strong_induction:
     cbv_value (erase_term ts) ->
     [[ Θ;
         (p, T_equiv (fvar y term_var) (tfix T ts)) ::
-        (y, T_forall (T_refine T_nat (annotated_tlt (lvar 0 term_var) (fvar n term_var))) T) ::
+        (y, T_forall (T_refine T_nat (binary_primitive Lt (lvar 0 term_var) (fvar n term_var))) T) ::
         (n, T_nat) ::
         Γ ⊨
         open 0 (open 1 ts (fvar n term_var)) (fvar y term_var) :
