ErasedEquivalentPrimitive.v
@@ -1,16 +1,17 @@
 Require Export SystemFR.ErasedPrimitive.
+Require Import Coq.Strings.String.
 
 
 Lemma reducible_values_primitive_EqEquiv1:
-  forall ρ v1 v2,
-    [ ρ ⊨ v1 : T_nat ]v ->
-    [ ρ ⊨ v2 : T_nat ]v ->
+  forall v1 v2,
+    cbv_value v1 ->
+    cbv_value v2 ->
     [ binary_primitive Eq v1 v2 ≡ ttrue ] ->
     [ v1 ≡ v2 ].
 Proof.
   unfold reduces_to; intros; repeat simp_red; repeat is_nat_value_buildable; steps.
-  apply_anywhere equivalent_true; last_step_binary_primitive.
-  rewrite PeanoNat.Nat.eqb_eq in *; subst.
+  apply_anywhere equivalent_true. last_step_binary_primitive.
+   rewrite PeanoNat.Nat.eqb_eq in *; subst.
   unfold equivalent_terms; steps; eauto with erased values wf fv.
 Qed.
 
@@ -18,31 +19,28 @@ Opaque Coq.Init.Wf.Fix_F.
 Opaque  Subterm.FixWf.
 
 Lemma reducible_primitive_EqEquiv1:
-  forall ρ t1 t2,
-    valid_interpretation ρ ->
-    [ ρ ⊨ t1 : T_nat ] ->
-    [ ρ ⊨ t2 : T_nat ] ->
+  forall t1 t2,
     [ binary_primitive Eq t1 t2 ≡ ttrue ] ->
     [ t1 ≡ t2 ].
 Proof.
-  intros;
-    repeat steps || simp_red || is_nat_value_buildable || unfold closed_term in * || top_level_unfold reduces_to ; eauto with erased wf.
-  eapply equivalent_trans; [
-    apply equivalent_star; eauto with erased wf fv | idtac].
+  steps.
+  pose proof H.
+  apply_anywhere equivalent_true.
+  t_invert_star; eauto with values. steps.
+  eapply equivalent_trans; [ top_level_unfold equivalent_terms;
+    apply equivalent_star; eauto with erased wf fv; t_closer | idtac].
   eapply equivalent_sym, equivalent_trans; [equivalent_star | idtac].
   apply equivalent_sym.
-  eapply (reducible_values_primitive_EqEquiv1 ρ); unfold reduces_to; steps;
+  eapply reducible_values_primitive_EqEquiv1; unfold reduces_to; steps;
     autorewrite with reducible_values; eauto with cbvlemmas values reducible_values.
   eapply equivalent_trans; [idtac | eauto using equivalent_refl with fv erased values].
   apply equivalent_sym, equivalent_star;
-    repeat steps || list_utils ; eauto with wf erased fv.
+    repeat steps || list_utils || top_level_unfold equivalent_terms ; eauto with wf erased fv.
   apply star_smallstep_binary_primitive; eauto with values.
 Qed.
 
 Lemma open_reducible_primitive_EqEquiv1:
   forall Θ Γ t1 t2,
-    [Θ; Γ ⊨ t1 : T_nat] ->
-    [Θ; Γ ⊨ t2 : T_nat] ->
     [Θ; Γ ⊨ binary_primitive Eq t1 t2 ≡ ttrue ] ->
     [Θ; Γ ⊨ t1 ≡ t2].
 Proof. unfold open_reducible, open_equivalent; steps;
@@ -118,16 +116,58 @@ Proof. unfold open_reducible, open_equivalent; steps;
 Qed.
 Hint Resolve open_reducible_primitive_EqEquiv2: primitives.
 
+Lemma open_reducible_primitive_Eq_args:
+  forall Θ Γ t1 t2,
+    [Θ; Γ ⊨ binary_primitive Eq t1 t2 ≡ ttrue ] ->
+    [Θ; Γ ⊨ t1 : T_nat] /\ [Θ; Γ ⊨ t2 : T_nat].
+Proof.
+  intros. unfold open_equivalent, open_reducible in *; steps; specialize (H ρ lterms); intuition auto;
+  assert (closed_term (psubstitute t2 lterms term_var)) by
+      (unfold equivalent_terms, closed_term, open_equivalent, open_reducible in *; repeat steps || list_utils);
+  assert (closed_term (psubstitute t1 lterms term_var)) by
+      (unfold equivalent_terms, closed_term, open_equivalent, open_reducible in *; repeat steps || list_utils);
+  apply_anywhere equivalent_true;
+  eapply_anywhere star_smallstep_binary_primitive_inv; eauto with values; steps;
+  step_inversion scbv_step; steps;
+  unfold reduces_to; steps; eauto with values smallstep;
+  eexists; split; eauto;
+  rewrite reducible_values_equation_4; apply is_nat_value_build_nat.
+Qed.
+
+
 Lemma open_reducible_primitive_EqSym:
   forall Θ Γ t1 t2,
-    [Θ; Γ ⊨ t1 : T_nat] ->
-    [Θ; Γ ⊨ t2 : T_nat] ->
     [Θ; Γ ⊨ binary_primitive Eq t1 t2 ≡ ttrue ] ->
     [Θ; Γ ⊨ binary_primitive Eq t2 t1 ≡ ttrue ].
 Proof.
   steps.
-  apply open_reducible_primitive_EqEquiv2; eauto.
+  apply open_reducible_primitive_EqEquiv2;
+    try solve [
+          apply_anywhere open_reducible_primitive_Eq_args; steps].
   assert ([Θ; Γ ⊨ t1 ≡ t2]). apply open_reducible_primitive_EqEquiv1; eauto.
   unfold open_equivalent in * ; steps ; eauto using equivalent_sym.
 Qed.
 Hint Resolve open_reducible_primitive_EqSym: primitives.
+
+Lemma reducible_values_primitive_Lt_sound:
+  forall a b, cbv_value a ->
+         cbv_value b ->
+         [ binary_primitive Lt a b ≡ ttrue] ->
+         tree_size a < tree_size b.
+Proof.
+  intros.
+  apply_anywhere equivalent_true. last_step_binary_primitive.
+  repeat rewrite tree_size_build_nat; steps. Psatz.lia.
+Qed.
+
+Ltac reducible_values_primitive_Lt_sound :=
+  match goal with
+  | H: binary_primitive Lt ?a ?b ~>* ttrue |- _ =>
+    cbv_value a; cbv_value b;
+    poseNew (Mark (a,b) "reducible_values_primitive_Lt_sound");
+    unshelve epose proof (reducible_values_primitive_Lt_sound a b _ _ H)
+  | H: [ binary_primitive Lt ?a ?b ≡ ttrue ] |- _ =>
+    cbv_value a; cbv_value b;
+    poseNew (Mark (a,b) "reducible_values_primitive_Lt_sound");
+    unshelve epose proof (reducible_values_primitive_Lt_sound a b _ _ _)
+  end.
